Add: +2

theories/Main.v
@@ -1470,7 +1470,7 @@ Defined.
 Definition trpt_cpq_u@{i j | }
   {A : Type@{i}} (P : A -> Type@{j}) {x y z : A}
   (p : Path@{i} x y) (q : Path@{i} y z) (u : P x)
-  : Path@{j} (trpt (conc p q) u) u.
+  : Path@{j} (trpt (conc p q) u) (trpt q (trpt p u)).
 Proof.
   refine (match q with idpath => _ end).
   refine (match p with idpath => _ end).
@@ -1484,7 +1484,32 @@ Definition trpt_p_trpt_vp_u@{i j | }
   (p : Path@{i} x y) (u : P y)
   : Path@{j} (trpt p (trpt (inv p) u)) u.
 Proof.
+  refine (conc _ (_ : Path@{j} (trpt (conc (inv p) p) u) _)).
+  -
+    exact (inv (trpt_cpq_u P (inv p) p u)).
+  -
+  refine (conc _ (_ : Path@{j} (trpt idpath u) _)).
+  +
+    exact (ap (fun p => trpt p u) (conc_vp_p p)).
+  +
+  simpl trpt.
+  exact idpath.
+Defined.
+
+(** trpt_inv_p_trpt_p_u です。 *)
+Definition trpt_vp_trpt_p_u@{i j | }
+  {A : Type@{i}} (P : A -> Type@{j}) {x y : A}
+  (p : Path@{i} x y) (u : P x)
+  : Path@{j} (trpt (inv p) (trpt p u)) u.
+Proof.
   refine (conc _ (_ : Path@{j} (trpt (conc p (inv p)) u) _)).
   -
-    refine (inv _).
-    refine (trpt_cpq_u P p (inv p) u).
+    exact (inv (trpt_cpq_u P p (inv p) u)).
+  -
+  refine (conc _ (_ : Path@{j} (trpt idpath u) _)).
+  +
+    exact (ap (fun p => trpt p u) (conc_p_vp p)).
+  +
+  simpl trpt.
+  exact idpath.
+Defined.
